Refactor proof stack-object to reduce compilation load

theories/case_studies/stack_object/stack_object_helpers.v
@@ -29,6 +29,120 @@ Section stack_object_helpers.
   (*   iMod (monotone_close_list_region with "[] [$Hsts $Hr $Htemp]") as "[$ $]"; auto. *)
   (* Qed. *)
 
+  Definition so_object_addresses (b e : Addr) :=
+    finz.seq_between b e.
+
+  Definition so_object_temporaries (W : WORLD) (b e : Addr) :=
+    filter
+      (fun a => std W !! a = Some Temporary)
+      (so_object_addresses b e).
+
+  Definition so_object_permanents (W : WORLD) (b e : Addr) :=
+    filter
+      (fun a => std W !! a = Some Permanent)
+      (so_object_addresses b e).
+
+  Definition so_revoked_without_object
+      (W : WORLD) (b e : Addr) (l : list Addr) :=
+    filter
+      (fun a => a ∉ so_object_temporaries W b e)
+      l.
+
+  Lemma NoDup_subset_filter_membership
+      {A} `{EqDecision0 : EqDecision A} (xs ys : list A) :
+    NoDup xs ->
+    NoDup ys ->
+    xs ⊆ ys ->
+    xs ≡ₚ filter (fun y => y ∈ xs) ys.
+  Proof.
+    intros Hnodup_xs Hnodup_ys Hsubset.
+    generalize dependent xs.
+    induction ys as [|y ys]; intros xs Hnodup_xs Hsubset.
+    - destruct xs; last set_solver.
+      done.
+    - cbn.
+      apply NoDup_cons in Hnodup_ys as [Hy_ys Hnodup_ys].
+      destruct (decide (y ∈ xs)) as [Hy_xs | Hy_xs].
+      + apply elem_of_Permutation in Hy_xs as [xs' Hxs].
+        setoid_rewrite Hxs in Hnodup_xs.
+        apply NoDup_cons in Hnodup_xs as [Hy_xs' Hnodup_xs'].
+        setoid_rewrite Hxs in Hsubset.
+        setoid_rewrite Hxs at 1.
+        assert (xs' ⊆ ys) as Hsubset'.
+        { intros x Hx.
+          assert (x ≠ y) by (intro; simplify_eq; done).
+          apply (list_elem_of_further _ y) in Hx.
+          apply Hsubset in Hx.
+          apply elem_of_cons in Hx as [Hx|Hx]; auto.
+          done.
+        }
+        eapply IHys in Hsubset'; eauto.
+        apply Permutation_cons; first done.
+        rewrite Hsubset'.
+        clear -Hnodup_ys Hxs Hy_ys.
+        induction ys; cbn; first done.
+        apply not_elem_of_cons in Hy_ys as [Hy_a Hy_ys].
+        apply NoDup_cons in Hnodup_ys as [_ Hnodup_ys].
+        destruct (decide (a ∈ xs')) as [Ha|Ha].
+        * apply (list_elem_of_further _ y) in Ha.
+          setoid_rewrite <- Hxs in Ha.
+          rewrite decide_True; last done.
+          rewrite IHys; auto.
+        * rewrite decide_False; first (rewrite IHys; auto).
+          intros Ha'.
+          setoid_rewrite Hxs in Ha'.
+          apply elem_of_cons in Ha' as [Ha'|?]; auto.
+      + eapply IHys; auto.
+        intros x Hx.
+        assert (x ≠ y) by (intro; simplify_eq; done).
+        apply Hsubset in Hx.
+        apply elem_of_cons in Hx as [Hx|Hx]; auto.
+        done.
+  Qed.
+
+  Lemma so_object_addresses_partition W b e :
+    Forall
+      (fun a =>
+         std W !! a = Some Permanent \/
+         std W !! a = Some Temporary)
+      (so_object_addresses b e) ->
+    so_object_addresses b e
+      ≡ₚ so_object_permanents W b e ++
+          so_object_temporaries W b e.
+  Proof.
+    intros Hstates.
+    rewrite /so_object_permanents /so_object_temporaries
+      /so_object_addresses in Hstates |- *.
+    generalize (finz.seq_between b e), Hstates.
+    clear Hstates.
+    induction l; intros Hl; cbn; first done.
+    apply Forall_cons in Hl as [Ha Hl].
+    apply IHl in Hl.
+    destruct Ha as [Ha | Ha].
+    - assert (std W !! a <> Some Temporary) as Ha'
+        by (intro; simplify_map_eq).
+      rewrite (decide_True _ _ Ha); auto.
+      rewrite (decide_False _ _ Ha'); auto.
+      cbn. rewrite -Hl. done.
+    - assert (std W !! a <> Some Permanent) as Ha'
+        by (intro; simplify_map_eq).
+      rewrite (decide_True _ _ Ha); auto.
+      rewrite (decide_False _ _ Ha'); auto.
+      cbn. rewrite -Permutation_middle -Hl. done.
+  Qed.
+
+  Lemma so_object_temporaries_NoDup W b e :
+    NoDup (so_object_temporaries W b e).
+  Proof.
+    apply NoDup_filter, finz_seq_between_NoDup.
+  Qed.
+
+  Lemma so_object_permanents_NoDup W b e :
+    NoDup (so_object_permanents W b e).
+  Proof.
+    apply NoDup_filter, finz_seq_between_NoDup.
+  Qed.
+
   Lemma open_world_interp_list (W : WORLD) (C' : CmptName)
     (l : list (Addr * Perm * (WORLD * CmptName * Word → iProp Σ) * region_type))
     (l' : list Addr)
