theories/case_studies/stack_object/stack_object_spec_closure.v
@@ -6,6 +6,9 @@ From griotte Require Import
   switcher interp_switcher_call switcher_spec_call switcher_spec_return.
 From griotte Require Import world_ghost_theory stack_object_helpers world_std_revocation.
 From griotte Require Import stack_object.
+From griotte Require Import stack_object_spec_blocks.
+From griotte Require Import stack_object_spec_resources.
+From griotte Require Import stack_object_spec_repair.
 From griotte Require Import proofmode.
 
 Section SO.
@@ -162,15 +165,8 @@ Section SO.
     iDestruct (big_sepM_delete _ _ ca1 with "Hrmap") as "[Hca1 Hrmap]"; first by simplify_map_eq.
 
     (* Extract the imports *)
-    iDestruct (region_pointsto_cons with "Himports_main") as "[Himport_switcher Himports_main]".
-    { transitivity (Some (pc_b ^+ 1)%a); auto; solve_addr. }
-    { solve_addr. }
-    iDestruct (region_pointsto_cons with "Himports_main") as "[Himport_assert Himports_main]".
-    { transitivity (Some (pc_b ^+ 2)%a); auto; solve_addr. }
-    { solve_addr. }
-    iDestruct (region_pointsto_cons with "Himports_main") as "[Himport_C_f Himports_main]".
-    { transitivity (Some (pc_b ^+ 3)%a); auto; solve_addr. }
-    { solve_addr. }
+    iDestruct (so_main_imports_pointsto with "Himports_main") as
+      "(Himport_switcher & Himport_assert & Himport_C_f & Himports_main)"; eauto.
 
     iAssert (interp W0 C wca0) as "#Hinterp_wca0_W0".
     { iApply "Hinterp_rmap"; eauto.
@@ -236,434 +232,87 @@ Section SO.
     assert (related_sts_priv_world W0 W1) as
       Hrelated_priv_W0_W1 by eapply revoke_related_sts_priv_world.
 
-    (* Because the passed object has read permission,
-       all the addresses must be in the world, either Temporary or Permanent *)
-    iAssert ( ⌜ Forall (fun a => std W0 !! a = Some Permanent ∨ std W0 !! a = Some Temporary)
-                (finz.seq_between b e) ⌝)%I
-    as "%Hstd_state_be_W0".
-    { iDestruct (readAllowed_valid_cap with "Hinterp_wca0_W0" ) as "%Hbe_revoked"; auto.
-      iPureIntro.
-      clear -Hbe_revoked.
-      eapply Forall_impl; eauto; cbn.
-      intros a Ha.
-      destruct Ha as (ρ & Ha & Hρ).
-      destruct ρ; [ right | left |]; done.
-    }
+    set (la_be_temporaries := so_object_temporaries W0 b e).
+    set (la_be_permanents := so_object_permanents W0 b e).
+    (* Filter the addresses that are in Temporary state in [la_be_temporaries]. *)
+    set (l_revoked_W0_no_be :=
+      so_revoked_without_object W0 b e l_revoked_W0).
 
-    (* Filter the addresses that are in Temporary state in [la_be_temporaries]
-       and the ones that are in Permanent state in [la_be_permanents] *)
-    set (la_be_temporaries := filter (fun a => std W0 !! a = Some Temporary) (finz.seq_between b e)).
-    set (la_be_permanents := filter (fun a => std W0 !! a = Some Permanent) (finz.seq_between b e)).
-    assert ( (finz.seq_between b e) ≡ₚ la_be_permanents ++ la_be_temporaries ) as Hwca0_range.
-    { clear - Hstd_state_be_W0 Hstd_state_be_W0.
-      subst la_be_permanents la_be_temporaries.
-      generalize (finz.seq_between b e), Hstd_state_be_W0.
-      clear Hstd_state_be_W0 b e .
-      induction l; intros Hl; cbn; first done.
-      apply Forall_cons in Hl as [Ha Hl]
-      ; apply IHl in Hl
-      ; destruct Ha as [Ha | Ha]
-      ; [ assert (W0.1 !! a ≠ Some Temporary) as Ha' by (intro ; simplify_map_eq)
-        | assert (W0.1 !! a ≠ Some Permanent) as Ha' by (intro ; simplify_map_eq) ]
-      ; rewrite (decide_True _ _ Ha); auto; rewrite (decide_False _ _ Ha'); auto
-      ; cbn ; [|rewrite -Permutation_middle] ; rewrite -Hl; done.
+    assert (la_be_temporaries ⊆ l_revoked_W0) as Htemps_subset.
+    { intros x Hx.
+      subst la_be_temporaries.
+      apply list_elem_of_filter in Hx as [Hx Hx_be].
+      apply (Hl_revoked_W0_temporaries x) in Hx.
+      apply elem_of_app in Hx as [Hx|Hx]; first done.
+      rewrite elem_of_disjoint in Hno_overlap.
+      exfalso; eapply Hno_overlap; eauto.
     }
-
-    (* Filter out of [l_revoked_W0] the addresses that are [la_be_temporaries]
-       and those that are not. *)
-    set (l_revoked_W0_no_be := filter (fun a => a ∉ la_be_temporaries) l_revoked_W0).
     assert (
-       la_be_temporaries ≡ₚ filter (fun a => a ∈ la_be_temporaries) l_revoked_W0
-      ) as Hla_be_temporaries_l.
-    {
-      clear -Hl_revoked_W0_nodup Hl_revoked_W0_temporaries Hno_overlap.
-      assert (la_be_temporaries ⊆ l_revoked_W0).
-      {
-        intros a Ha.
-        subst la_be_temporaries.
-        apply list_elem_of_filter in Ha as [Ha Ha_be].
-        apply (Hl_revoked_W0_temporaries a) in Ha.
-        apply elem_of_app in Ha as [Ha|Ha]; first done.
-        rewrite elem_of_disjoint in Hno_overlap.
-        exfalso; eapply Hno_overlap; eauto.
-      }
-      apply NoDup_app in Hl_revoked_W0_nodup as (Hnodup_l & _ & _).
-      assert (NoDup la_be_temporaries) as Hnodup_la_be_temporaries.
-      { subst la_be_temporaries. apply NoDup_filter, finz_seq_between_NoDup. }
-      (* can the proofs below be a lemma instead? *)
-      generalize la_be_temporaries, H, Hnodup_la_be_temporaries; intros l' Hl' Hnodup_l'.
-      clear -Hl' Hnodup_l Hnodup_l'.
-      generalize dependent l'.
-      induction l_revoked_W0 as [|a l_revoked_W0]; intros l' Hl' Hnodup_l'.
-      + destruct l' ; last set_solver.
-        done.
-      + cbn.
-        apply NoDup_cons in Hnodup_l as [Ha_l Hnodup_l].
-        destruct (decide (a ∈ l')) as [Ha_l' | Ha_l'].
-        * apply elem_of_Permutation in Ha_l' as [l0 Ha_l'].
-          setoid_rewrite Ha_l' in Hnodup_l'.
-          apply NoDup_cons in Hnodup_l' as [Ha_l0 Hnodup_l0].
-          setoid_rewrite Ha_l' in Hl'.
-          setoid_rewrite Ha_l' at 1.
-          assert (l0 ⊆ l_revoked_W0).
-          { clear -Ha_l Hl' Ha_l0.
-            intros x Hx.
-            assert (x ≠ a) by (intro; simplify_eq; done).
-            apply (list_elem_of_further _ a) in Hx.
-            apply Hl' in Hx.
-            apply elem_of_cons in Hx as [Hx|Hx]; auto.
-            done.
-          }
-          eapply (IHl_revoked_W0) in H; eauto.
-          apply Permutation_cons; first done.
-          rewrite H.
-          clear -Hnodup_l Ha_l' Ha_l.
-          induction l_revoked_W0; cbn; first done.
-          apply not_elem_of_cons in Ha_l as [Ha_a0 Ha_l].
-          apply NoDup_cons in Hnodup_l as [_ Hnodup_l].
-          destruct ( decide (a0 ∈ l0) ) as [Ha0|Ha0].
-          ** apply (list_elem_of_further _ a) in Ha0.
-             setoid_rewrite <- Ha_l' in Ha0.
-             rewrite decide_True; last done.
-             rewrite IHl_revoked_W0; auto.
-          ** rewrite decide_False; first (rewrite IHl_revoked_W0; auto).
-             intros Ha0'.
-             setoid_rewrite Ha_l' in Ha0'.
-             apply elem_of_cons in Ha0' as [Ha0'|?]; auto.
-        * eapply IHl_revoked_W0; auto.
-          clear -Hl' Ha_l Ha_l'.
-          intros x Hx.
-          assert (x ≠ a) by (intro; simplify_eq; done).
-          apply Hl' in Hx.
-          apply elem_of_cons in Hx as [Hx|Hx]; auto.
-          done.
+      la_be_temporaries
+        ≡ₚ filter (fun a => a ∈ la_be_temporaries) l_revoked_W0
+    ) as Hla_be_temporaries_l.
+    { apply NoDup_subset_filter_membership.
+      - apply so_object_temporaries_NoDup.
+      - apply NoDup_app in Hl_revoked_W0_nodup as [? _]. done.
+      - exact Htemps_subset.
     }
-    assert ( l_revoked_W0 ≡ₚ la_be_temporaries ∪ l_revoked_W0_no_be) as Hl_wca0_l'.
+    assert (
+      l_revoked_W0 ≡ₚ la_be_temporaries ++ l_revoked_W0_no_be
+    ) as Hl_wca0_l'.
     { subst l_revoked_W0_no_be.
       rewrite {1}Hla_be_temporaries_l.
       apply filter_complement_list.
     }
-    (* Eliminate the later of [RevokedResources] *)
-    iDestruct (lc_fupd_elim_later with "[$] [$Hl_revoked_W0]") as ">Hl_revoked_W0".
-    iEval (setoid_rewrite Hl_wca0_l') in "Hl_revoked_W0".
-    iDestruct (RevokedResources_app with "Hl_revoked_W0") as "[Hrevoked_la_be_temporaries Hrevoked_l_revoked_W0_no_be]".
-
-    (* Open the world for the Permanent addresses [la_be_permanents]:
-     - get the list of predicates [φs] and [rel] from the validity predicate of [wca0]
-     - open the world
-     - change the shape of the resources obtained from the open world in a more usable way
-     *)
-    (* rewrite region_open_nil. *)
-    iDestruct (read_allowed_inv_full_cap with "Hinterp_wca0_W0") as "Hinterp_wca0_invs"; auto.
-    iAssert (
-        ∃ (wca0_invs : list (finz MemNum * Perm * (WORLD * CmptName * Word → iProp Σ) * region_type)),
-          ⌜ (λ '(a, _, _, _), a) <$> wca0_invs = la_be_permanents ⌝ ∗
-          ⌜ Forall (λ '(a, _, _, ρ), std W0 !! a = Some ρ ∧ ρ = Permanent) wca0_invs ⌝ ∗
-          ([∗ list] '(a, p, φ, _) ∈ wca0_invs, rel C a p φ) ∗
-          ⌜ Forall (λ '(_, _, φ, _), ∀ Wv : WORLD * CmptName * Word, Persistent (φ Wv)) wca0_invs⌝
-      )%I as "(%wca0_invs & %Hwca0_invs_perma & %Hwca0_invs_std_perma & Hrels_wca0 & %Hpers_wca0_invs)".
-    {
-      iDestruct "Hinterp_wca0_invs" as "-#Hinterp_wca0_invs".
-      iClear "#".
-      setoid_rewrite Hwca0_range.
-      iDestruct (big_sepL_app with "Hinterp_wca0_invs") as "[H _]".
-      iDestruct "H" as "#H".
-      assert (Forall (λ a : finz MemNum, W0.1 !! a = Some Permanent) la_be_permanents) as Hla_be_permanents.
-      { subst la_be_permanents.
-        clear.
-        induction (finz.seq_between b e); first done.
-        cbn.
-        destruct ( decide (W0.1 !! a = Some Permanent) ); last done.
-        apply Forall_cons; split ;auto.
-      }
-      generalize la_be_permanents, Hla_be_permanents.
-      clear; intros l Hl.
-      iInduction (l) as [|a l] "IH".
-      + iExists []; cbn.
-        repeat (iSplit; iPureIntro; done).
-      + apply Forall_cons in Hl as [Ha Hl].
-        cbn.
-        iDestruct "H" as "[ (%p'& %P' & %Hpermflow & %HpersP
-                              & HrelP & Hzcond & Hrcond & Hwcond & Hmono) H ]".
-        iDestruct ("IH" with "[%] [$]") as "(%invs & %Hl_ & %Hperma & #Hrels & %Hpers )"; auto.
-        iExists (( (a,p',safeC P'), Permanent)::invs).
-        iSplit; first iPureIntro.
-        { cbn; by rewrite Hl_. }
-        iSplit; first iPureIntro.
-        { apply Forall_cons; split; auto. }
-        iSplit; first cbn; iFrame "#".
-        iPureIntro.
-        apply Forall_cons; split; auto.
+    assert (
+      Forall
+        (fun a => std (revoke W0) !! a = Some Revoked)
+        la_be_temporaries
+    ) as Hrevoked_la_be_temporaries.
+    { apply Forall_forall. intros x Hx.
+      apply revoke_lookup_Monotemp.
+      apply Hl_revoked_W0_temporaries.
+      apply elem_of_app; left.
+      by apply Htemps_subset.
+    }
+    assert (
+      finz.seq_between csp_b csp_e ## la_be_temporaries
+    ) as Hstack_temps_disjoint.
+    { rewrite elem_of_disjoint in Hno_overlap |- *.
+      intros x Hx_stk Hx_temp.
+      eapply Hno_overlap.
+      - subst la_be_temporaries.
+        apply list_elem_of_filter in Hx_temp as [_ Hx_object].
+        exact Hx_object.
+      - exact Hx_stk.
     }
 
-    rewrite open_world_interp_empty.
-    iDestruct (open_world_interp_list with "[$Hrels_wca0 $Hworld_interp_C]") as
-      "(%wca0_lv_perma & Hworld_interp_C & Hsts_std_wca0 & Hla_be_permanents_lv & Hwca0_mono & Hwca0_φs
-     & %Hlength_wca0_lv & Hwca0_pO)".
-    { rewrite Hwca0_invs_perma.
-      subst la_be_permanents.
-      apply NoDup_filter, finz_seq_between_NoDup.
-    }
-    { rewrite Hwca0_invs_perma; set_solver+. }
-    { rewrite !Forall_forall in Hwca0_invs_std_perma |- *.
-      intros [ [ [  ] ] ] Hx; cbn in *; simplify_eq.
-      apply Hwca0_invs_std_perma in Hx.
-      destruct Hx as [_ ->]; done.
-    }
-    { cbn in *.
-      rewrite !Forall_forall in Hwca0_invs_std_perma |- *.
-      intros [ [ [  ] ] ] Hx; cbn in *; simplify_eq.
-      apply Hwca0_invs_std_perma in Hx.
-      destruct Hx as [Hx ->].
-      by apply revoke_lookup_Perm.
-    }
-    iAssert ( [∗ list] a;v ∈ la_be_permanents ; wca0_lv_perma, a ↦ₐ v )%I with "[Hla_be_permanents_lv]"
-      as "Hla_be_permanents_lv".
-    { iClear "#". clear -Hwca0_invs_perma.
-      iStopProof.
-      rewrite -Hwca0_invs_perma big_sepL2_fmap_l.
-      generalize dependent la_be_permanents; intros l Hl.
-      generalize dependent wca0_invs.
-      generalize dependent wca0_lv_perma.
-      induction l; iIntros (lv linvs Hl) "Hl".
-      + apply fmap_nil_inv in Hl; simplify_eq; done.
-      + apply fmap_cons_inv in Hl; simplify_eq.
-        destruct Hl as ( apφρ & l' & Ha & Hl' & Hl); cbn in *.
-        destruct apφρ as [ [ [] ] ]; simplify_eq; cbn.
-        iDestruct (big_sepL2_length with "Hl") as "%Hlen"
-        ; destruct lv ; simplify_eq.
-        cbn.
-        iDestruct "Hl" as "[$ Hl]".
-        iApply IHl; eauto.
-    }
-    assert (Forall (λ a : finz MemNum, (revoke W0).1 !! a = Some Revoked) la_be_temporaries) as
-      Hrevoked_la_be_temporaries.
-    { clear - Hl_wca0_l' Hl_revoked_W0.
-      rewrite /revoked_addresses in Hl_revoked_W0.
-      setoid_rewrite Hl_wca0_l' in Hl_revoked_W0.
-      apply Forall_app in Hl_revoked_W0 as [? ?].
-      auto.
-    }
-
-    (* Get the list of permissions, predicates and words for the [la_be_temporaries] *)
-    iAssert (
-        ∃ (lp : list Perm)
-          (lφ : list (WORLD * CmptName * Word → iPropI Σ) )
-          (lv : list Word),
-          ⌜ length lp = length la_be_temporaries ⌝
-          ∗ ⌜ length lφ = length la_be_temporaries ⌝
-          ∗ ⌜ length lv = length la_be_temporaries ⌝
-          ∗ ([∗ list] φ ∈ lφ, ⌜∀ Wv : WORLD * CmptName * Word, Persistent (φ Wv)⌝)
-          ∗ ([∗ list] a;pφ ∈ la_be_temporaries;(zip lp lφ), rel C a pφ.1 pφ.2)
-          ∗ ([∗ list] p ∈ lp, ⌜isO p = false⌝)
-          ∗ ([∗ list] a;v ∈ la_be_temporaries;lv, a ↦ₐ v)
-          ∗ ([∗ list] lpφ;v ∈ (zip lp lφ);lv,
-               (if isWL lpφ.1
-                then future_pub_mono C lpφ.2 v
-                else (if isDL lpφ.1 then future_pub_mono C lpφ.2 v else future_priv_mono C lpφ.2 v))
-            )
-          ∗ ([∗ list] φ;v ∈ lφ;lv, φ (W0,C,v)))%I
-      with "[Hrevoked_la_be_temporaries]"
-      as (lp lφ wca0_lv_temps)
-           "(%Hlen_lp & %Hlen_lφ & %Hlen_lv & Hlφ_pers & #Hlpφ_rels & HlpO & Hla_be_temporaries_lv & Hlpφ_mono & Hlφ_lv)".
-    { iClear "#".
-      generalize la_be_temporaries.
-      clear; intros l.
-      iInduction (l) as [| a l]; first (iExists [],[],[]; cbn; done).
-      iDestruct "Hrevoked_la_be_temporaries" as "[Ha Hl]".
-      iDestruct ("IHl" with "Hl") as "Hl".
-      iDestruct "Ha" as (p P HpersP) "[Hrel_a Ha]".
-      iDestruct "Ha" as (v) "(HpO & Hv & HP & HmonoP)".
-      iDestruct "Hl" as (lp lP lv) "(% & % & % & %Hpers_lP & Hrels & HpOs & Hvs & Hmonos & HPs)".
-      iExists (p::lp), (P::lP), (v::lv).
-      rewrite mono_temporary_eq.
-      iFrame.
-      iFrame "%".
-      iPureIntro.
-      cbn; lia.
-    }
-    iDestruct (big_sepL2_app with "Hla_be_permanents_lv Hla_be_temporaries_lv") as "Hwca0_lvs".
+    (* Get the list of permissions, predicates and words for the [la_be_temporaries]. *)
+    iMod (stack_object_open_region_for_checkints
+      W0 C p g b e a csp_b csp_e l_revoked_W0 stk_mem
+      with "[$Hinterp_wca0_W0 $Hworld_interp_C $Hl_revoked_W0 $Hstk $Hlc]")
+      as (wca0_lvs)
+        "(%Hwca0_lvs_length & %Hwca0_range & Hwca0_lvs & Hrestore_wca0)".
+    { split; eauto. }
+    { exact Hno_overlap. }
+    { exact Hp. }
 
     (* Apply the checkint specification*)
-    iApply (checkints_spec with "[- $HPC $Hca0 $Hcs1 $Hcs0 $Hwca0_lvs $Hcode]"); eauto.
-    { symmetry; auto. }
-    iSplitL; last ( iModIntro; iNext ; iIntros (?); done).
-    iNext ; iIntros "(HPC & Hca0 & Hcs0 & Hcs1 & Hwca0_lvs & %Hwca0_lvs_ints & Hcode & Hlc)".
+    iApply (checkints_spec
+      with "[- $HPC $Hca0 $Hcs1 $Hcs0 $Hwca0_lvs $Hcode]"); eauto.
+    { symmetry; exact Hwca0_range. }
+    iSplitL; last (iModIntro; iNext; iIntros (?); done).
+    iNext.
+    iIntros "(HPC & Hca0 & Hcs0 & Hcs1 & Hwca0_lvs
+              & %Hwca0_lvs_ints & Hcode & Hlc)".
     subst hcont; unfocus_block "Hcode" "Hcont" as "Hcode_main".
 
-    (* Close the world from the opened addresses [la_be_permanents] *)
-    iDestruct (big_sepL2_app' with "Hwca0_lvs") as "[Hla_be_permanents_lv Hla_be_temporaries_lv]".
-    { by rewrite Hlength_wca0_lv Hwca0_invs_perma. }
-    iAssert ( [∗ list] '(a0, _, _, _);v ∈ wca0_invs;wca0_lv_perma, a0 ↦ₐ v )%I with "[Hla_be_permanents_lv]"
-      as "Hla_be_permanents_lv".
-    { iClear "#". clear -Hwca0_invs_perma.
-      iStopProof.
-      rewrite -Hwca0_invs_perma big_sepL2_fmap_l.
-      generalize dependent la_be_permanents; intros l Hl.
-      generalize dependent wca0_invs.
-      generalize dependent wca0_lv_perma.
-      induction l; iIntros (lv linvs Hl) "Hl".
-      + apply fmap_nil_inv in Hl; simplify_eq; done.
-      + apply fmap_cons_inv in Hl; simplify_eq.
-        destruct Hl as ( apφρ & l' & Ha & Hl' & Hl); cbn in *.
-        destruct apφρ as [ [ [] ] ]; simplify_eq; cbn.
-        iDestruct (big_sepL2_length with "Hl") as "%Hlen"
-        ; destruct lv ; simplify_eq.
-        cbn.
-        iDestruct "Hl" as "[$ Hl]".
-        iApply IHl; eauto.
-    }
-
-    iDestruct (close_world_interp_list W1 C wca0_invs [] with
-             "[$Hworld_interp_C $Hsts_std_wca0 $Hla_be_permanents_lv $Hwca0_mono $Hwca0_φs $Hrels_wca0 $Hwca0_pO]"
-      ) as "Hworld_interp_C".
-    { by rewrite Hlength_wca0_lv length_fmap. }
-    { rewrite Hwca0_invs_perma. apply NoDup_filter, finz_seq_between_NoDup. }
-    { set_solver+. }
-    { rewrite !Forall_forall in Hwca0_invs_std_perma |- *.
-      intros [ [ [  ] ] ] Hx; cbn in *; simplify_eq.
-      apply Hwca0_invs_std_perma in Hx.
-      destruct Hx as [_ ->]; done.
-    }
-    { auto. }
-    rewrite -open_world_interp_empty.
-
-    (* Update the world and insert [la_be_temporaries].
-       It means that we need to prove that they are safe to share in the revoked world.
-       It's fine because they contain only integers.
-     *)
-    iAssert (▷ [∗ list] φ ∈ lφ, zcond (safeUC φ) C)%I as "#Hzcond_lφ".
-    { iClear "∗".
-      iDestruct "Hlpφ_rels" as "-#Hrels".
-      iDestruct "Hinterp_wca0_invs" as "-#Hinterp".
-      iClear "#".
-      setoid_rewrite Hwca0_range.
-      iDestruct (big_sepL_app with "Hinterp") as "[_ #Hinterp]".
-      generalize la_be_temporaries, Hlen_lp, Hlen_lφ.
-      clear.
-      intros l Hlen_lp Hlen_lφ.
-      iInduction (l) as [|a l] "IH" forall (lp lφ Hlen_lp Hlen_lφ).
-      all: destruct lφ; simplify_eq.
-      all: destruct lp; simplify_eq.
-      + done.
-      + cbn.
-        iDestruct "Hinterp" as "[(%p' & %P' & _ & _ & Hrel' & Hzcond & _) Hinterp]".
-        iDestruct "Hrels" as "[Hrel #Hrels]".
-        iDestruct (rel_agree  with "[$Hrel $Hrel']") as "[_ #Heq]".
-        iSplitL "Heq"; last iApply "IH"; eauto.
-        iNext.
-        iIntros (???) "!> H"; cbn.
-        iDestruct ("Heq" $! (W1, C, WInt z)) as "-#Heq0".
-        iDestruct ("Heq" $! (W2, C, WInt z)) as "-#Heq1".
-        (* FIXME: for some reason, I cant rewrite Heq0 and Heq1... *)
-        iDestruct (internal_eq_iff with "Heq1") as "[_ Heq1]".
-        iDestruct (internal_eq_iff with "Heq0") as "[Heq0 _]".
-        iApply "Heq1".
-        iDestruct ("Heq0" with "H") as "H".
-        iApply "Hzcond"; eauto.
-    }
-    iDestruct "Hlc" as "[Hlc' Hlc]".
-    iDestruct (lc_fupd_elim_later with "[$Hlc'] [$Hzcond_lφ]") as ">Hzcond_lφ'".
-    iAssert (
-        [∗ list] φ;v ∈ lφ;wca0_lv_temps, φ (W1, C, v)
-      )%I with "[Hlφ_lv Hzcond_lφ']" as "Hlφ_lv".
-    { iClear "#".
-      apply Forall_app in Hwca0_lvs_ints as [_ Hl].
-      generalize wca0_lv_temps, Hl, Hlen_lv.
-      generalize la_be_temporaries, Hlen_lp, Hlen_lφ.
-      clear.
-      intros la Hlen_lp Hlen_lφ lv Hl_ints Hlen_lv.
-      iInduction (la) as [|a la] "IH" forall (lp lφ lv Hlen_lp Hlen_lφ Hlen_lv Hl_ints).
-      all: destruct lφ; simplify_eq.
-      all: destruct lp; simplify_eq.
-      all: destruct lv; simplify_eq.
-      + done.
-      + cbn.
-        iDestruct "Hlφ_lv" as "[Hb Hlb]".
-        iDestruct "Hzcond_lφ'" as "[#Hz Hzl]".
-        apply Forall_cons in Hl_ints as [ [z ->] Hl_ints].
-        iSplitL "Hb Hz"; last (iApply ("IH" with "[] [] [] [] [$] [$]") ; eauto).
-        rewrite /zcond.
-        iSpecialize ("Hz" $! W0 W1 z).
-        cbn.
-        iApply "Hz"; auto.
-    }
-    iDestruct (big_sepL2_disjoint with "[$Hstk $Hla_be_temporaries_lv]") as "%".
-    iAssert (
-        ([∗ list] a ∈ la_be_temporaries,
-           ∃ p φ, ⌜forall Wv, Persistent (φ Wv)⌝ ∗ temp_resources W1 C φ a p ∗ rel C a p φ)
-      )%I with "[Hlφ_pers HlpO Hlpφ_mono Hla_be_temporaries_lv Hlφ_lv]" as "Hla_be_temporaries_closing_resources".
-    { iDestruct "Hlpφ_rels" as "-#Hlpφ_rels".
-      iClear "#".
-      assert (Forall (λ w : Word, ∃ z : Z, w = WInt z) wca0_lv_temps) as Hlvs_temp_int.
-      { clear -Hwca0_lvs_ints.
-        by apply Forall_app in Hwca0_lvs_ints as [??].
-      }
-      clear -Hlen_lp Hlen_lφ Hlen_lv.
-      generalize dependent la_be_temporaries; intros l Hlen_lp Hlen_lφ Hlen_lv.
-      generalize wca0_lv_temps Hlen_lv; intros lv.
-      clear Hlen_lv wca0_lv_temps; intros Hlen_lv.
-      iRename "Hla_be_temporaries_lv" into "Hlv".
-      iInduction (l) as [|a l] "IH" forall (lφ lp lv Hlen_lp Hlen_lφ Hlen_lv); first done.
-      destruct lv as [|v lv]; cbn in Hlen_lv; simplify_eq.
-      destruct lφ as [|φ lφ]; cbn in Hlen_lφ; simplify_eq.
-      destruct lp as [|p lp]; cbn in Hlen_lp; simplify_eq.
-      cbn in *.
-      iDestruct "Hlφ_pers" as "[Hlφ_pers_a Hlφ_pers]".
-      iDestruct "HlpO" as "[HlpO_a HlpO]".
-      iDestruct "Hlpφ_mono" as "[Hlpφ_mono_a Hlpφ_mono]".
-      iDestruct "Hlv" as "[Hlv_a Hlv]".
-      iDestruct "Hlφ_lv" as "[Hlφ_lv_a Hlφ_lv]".
-      iDestruct "Hlpφ_rels" as "[Hlpφ_rels_a Hlpφ_rels]".
-      iFrame.
-      iApply ("IH" $! lφ lp lv with "[%] [%] [%] [$] [$] [$] [$] [$] [$]"); eauto.
-    }
-    iMod (world_interp_restore_world W1 W1 C la_be_temporaries with
-      "[$Hworld_interp_C] [ Hla_be_temporaries_closing_resources ]") as "Hworld_interp_C".
-    { apply close_list_related_sts_pub. }
-    { iClear "#".
-      iApply (big_sepL_impl with "Hla_be_temporaries_closing_resources").
-      iModIntro; iIntros (k ka Hka) "(%&%&$&(%&$&$&?&$)&$)".
-      by rewrite mono_temporary_eq.
-    }
-    set ( W2 := (close_list la_be_temporaries W1)).
-
-    (* The passed object is safe to share in the world [W2] *)
-    iAssert (interp W2 C (WCap p g b e (finz.max b e)))%I as "#Hinterp_wca0_W2".
-    {
-      iEval (rewrite fixpoint_interp1_eq interp1_eq).
-      iEval (rewrite fixpoint_interp1_eq interp1_eq) in "Hinterp_wca0_W0".
-      destruct (isO p); first done.
-      destruct (has_sreg_access p); first done.
-      iDestruct "Hinterp_wca0_W0" as "[ Hinterp $ ]".
-      iClear "∗".
-      iApply (big_sepL_impl with "Hinterp").
-      iModIntro.
-      iIntros (k x Hx) "(%px & %Px & %Hpx_flow & %Hpers_Px & Hrelx
-                             & Hzcondx & Hrcondx & Hwcondx & Hmonox & %Hstatex)".
-      iFrame "∗%".
-      apply list_elem_of_lookup_2 in Hx.
-      rewrite Forall_forall in Hstd_state_be_W0.
-      assert (std W0 !! x = std W2 !! x) as Hxeq.
-      { destruct (Hstd_state_be_W0 x Hx) as [Hx' | Hx']; rewrite Hx'; symmetry.
-        * rewrite close_list_lookup_not_in.
-          { cbn.
-            by apply revoke_lookup_Perm.
-          }
-          intro Hcontra.
-          apply list_elem_of_filter in Hcontra as [ hcontra _ ].
-          by rewrite hcontra in Hx'.
-        * apply close_list_lookup_in; auto; last (apply list_elem_of_filter; split; done).
-          cbn; apply revoke_lookup_Monotemp; auto.
-      }
-      iSplitL "Hmonox".
-      + rewrite /monoReq.
-        by rewrite Hxeq.
-      + iPureIntro.
-        destruct (isWL p); rewrite !/region_state_nwl !/region_state_pwl in Hstatex |- *
-        ; rewrite -Hxeq; done.
-    }
-
+    set (W2 := close_list la_be_temporaries W1).
+    iDestruct "Hlc" as "[Hlc_restore Hlc]".
+    (* Close the world from the opened addresses [la_be_permanents]. *)
+    iMod ("Hrestore_wca0" with "[$Hwca0_lvs $Hlc_restore]")
+      as "(Hworld_interp_C & Hrevoked_l_revoked_W0_no_be
+           & Hstk & #Hinterp_wca0_W2)".
+    { iPureIntro. exact Hwca0_lvs_ints. }
 
     (* ------------------------------------------------------- *)
     (* ------------------ BLOCK 7: ALLOC_SO ------------------ *)
@@ -671,73 +320,17 @@ Section SO.
     focus_block 7 "Hcode_main" as a_alloc_so Ha_alloc_so "Hcode" "Hcont"; iHide "Hcont" as hcont
     ; clear dependent Ha_checkints.
 
-    (* Store csp so_secret; *)
-    destruct ( decide ((csp_b < csp_e)%a) ) as [Hcsp_size|Hcsp_size]; cycle 1.
-    {
-      iInstr_lookup "Hcode" as "Hi" "Hcode".
-      wp_instr.
-      iApply (wp_store_fail_z with "[$HPC $Hi $Hcsp]"); try solve_pure.
-      { rewrite /withinBounds; solve_addr+Hcsp_size. }
-      iIntros "!> _".
-      wp_pure; wp_end; iIntros (?); done.
-    }
-    iDestruct (big_sepL2_length with "Hstk") as %Hstklen.
-    rewrite finz_seq_between_length in Hstklen.
-    rewrite finz_dist_S in Hstklen; last solve_addr+Hcsp_size.
-    destruct stk_mem as [|w0 stk_mem]; simplify_eq.
-    assert (is_Some (csp_b + 1)%a) as [a_stk1 Hastk1];[solve_addr+Hcsp_size|].
-    iDestruct (region_pointsto_cons with "Hstk") as "[Hastk0 Hstk]"; eauto.
-    { solve_addr+Hcsp_size Hastk1. }
-    iInstr "Hcode".
-    { rewrite /withinBounds; solve_addr+Hcsp_size. }
-    (* Lea csp 1; *)
-    iInstr "Hcode".
-    (* Mov ca1 csp; *)
-    iInstr "Hcode".
-    (* GetA cs0 ca1; *)
-    iInstr "Hcode".
-    (* Add cs1 cs0 1; *)
-    iInstr "Hcode".
-    (* Subseg ca1 cs0 cs1; *)
-    destruct ( decide ((a_stk1 < csp_e)%a) ) as [Hcsp_size'|Hcsp_size']; cycle 1.
-    {
-      destruct (z_to_addr (a_stk1 + 1))%a as [a_stk2|] eqn:Hastk2; cycle 1.
-      + iInstr_lookup "Hcode" as "Hi" "Hcode".
-        wp_instr.
-        iApply (wp_subseg_fail_src2_nonaddr with "[$HPC $Hi $Hca1 $Hcs0 $Hcs1]"); try solve_pure.
-        iIntros "!> _".
-        wp_pure; wp_end; iIntros (?); done.
-      + iInstr_lookup "Hcode" as "Hi" "Hcode".
-        wp_instr.
-        iApply (wp_subseg_fail_not_iswithin_cap with "[$HPC $Hi $Hca1 $Hcs0 $Hcs1]"); try solve_pure.
-        { eauto. }
-        {
-          assert (csp_e < a_stk2)%a as Hcsp_e_stk2 by solve_addr+Hastk1 Hcsp_size Hcsp_size' Hastk2.
-          rewrite /isWithin.
-          apply andb_false_iff.
-          right.
-          solve_addr+Hcsp_e_stk2.
-        }
-        iIntros "!> _".
-        wp_pure; wp_end; iIntros (?); done.
-    }
-    iDestruct (big_sepL2_length with "Hstk") as %Hstklen'.
-    rewrite finz_seq_between_length in Hstklen'.
-    rewrite finz_dist_S in Hstklen'; last solve_addr+Hcsp_size'.
-    destruct stk_mem as [|w1 stk_mem]; simplify_eq.
-    assert (is_Some (a_stk1 + 1)%a) as [a_stk2 Hastk2];[solve_addr+Hcsp_size'|].
-    iDestruct (region_pointsto_cons with "Hstk") as "[Hastk1 Hstk]"; eauto.
-    { solve_addr+Hcsp_size Hastk1 Hcsp_size' Hastk2. }
-    iInstr "Hcode".
-    { transitivity (Some (a_stk2)%a); auto.
-      solve_addr+Hastk2.
-    }
-    { solve_addr+Hcsp_size Hastk1 Hcsp_size' Hastk2. }
-    (* Store ca1 0; *)
-    iInstr "Hcode".
-    { solve_addr+Hcsp_size Hastk1 Hcsp_size' Hastk2. }
-    (* Lea csp 1; *)
-    iInstr "Hcode".
+    iApply (stack_object_alloc_block_spec
+              with "[- $HPC $Hcsp $Hca1 $Hcs0 $Hcs1 $Hstk $Hcode]"); eauto.
+    iNext.
+    iIntros (a_stk1 a_stk2 w0 w1 stk_mem')
+      "(%Hastk1 & %Hastk2 & %Hastk_bounds & %Hstk_mem
+       & HPC & Hcsp & Hca1 & Hcs0 & Hcs1
+       & Hastk0 & Hastk1 & Hstk & Hcode)".
+    destruct Hastk_bounds as (Hcsp_astk1 & Hastk1_astk2 & Hastk2_csp_e).
+    assert (csp_b < csp_e)%a as Hcsp_size by solve_addr.
+    assert (a_stk1 < csp_e)%a as Hcsp_size' by solve_addr.
+    subst stk_mem; rename stk_mem' into stk_mem.
     subst hcont; unfocus_block "Hcode" "Hcont" as "Hcode_main".
 
     (* --------------------------------------------------- *)
@@ -758,12 +351,10 @@ Section SO.
     (* --------------------------------------------------- *)
 
     focus_block 9 "Hcode_main" as a_call Ha_call "Hcode" "Hcont"; iHide "Hcont" as hcont; clear dependent Ha_fetch.
-    (* Mov cs0 cra *)
-    iInstr "Hcode".
-    (* Mov cs1 ct1 *)
-    iInstr "Hcode".
-    (* Jalr cra ct0 *)
-    iInstr "Hcode" with "Hl".
+    iApply (stack_object_call_block_spec
+              with "[- $HPC $Hcra $Hct0 $Hct1 $Hcs0 $Hcs1 $Hcode]"); eauto.
+    iNext.
+    iIntros "(HPC & Hcra & Hct0 & Hct1 & Hcs0 & Hcs1 & Hcode)".
 
 
     (* and the hard part should be mostly done at that point *)
@@ -820,100 +411,36 @@ Section SO.
     { iApply "Hzeroed_rmap"; eauto.
       set_solver+.
     }
-    iAssert (
-        |={⊤}=> ([∗ list] a ∈ [a_stk1],
-           ∃ p φ, ⌜forall Wv, Persistent (φ Wv)⌝ ∗ temp_resources W2 C φ a p ∗ rel C a p φ)
-      )%I with "[Hastk1 Hlc]" as ">Hastk1_closing_resources".
-    { cbn.
-      iDestruct (read_allowed_inv _ _ a_stk1 with "Hinterp_W0_csp")
-        as "(%pastk1 & %Pastk1 &
-      %Hpastk1_rwl & %Hpers_Pastk1 & #Hrel_astk1
-      & Hzcond_Pastk1 & Hrcond_Pastk1 & Hwcond_Pastk1 & Hmono_Pastk1
-      )";auto.
-      { solve_addr+Hastk1 Hcsp_size'. }
-      replace (writeAllowed pastk1) with true.
-      2:{ symmetry; eapply writeAllowed_flowsto; eauto. }
-      iDestruct (lc_fupd_elim_later with "[$] [$Hwcond_Pastk1]") as ">#Hwcond_Pastk1'".
-      assert (isWL pastk1 = true) as Hpastk1_wl by (apply isWL_flowsto in Hpastk1_rwl;done).
-      iModIntro.
-      iSplitL; last done.
-      iExists pastk1, (safeC Pastk1).
-      iSplit; first iPureIntro.
-      { intros Wcv; apply Hpers_Pastk1. }
-      iSplit; last iFrame "#".
-      iFrame "Hastk1".
-      iSplit; first iPureIntro.
-      { by apply isWL_nonO. }
-      rewrite /monoReq !Hpastk1_wl.
-      iSplit.
-      + replace (W0.1 !! a_stk1) with (Some Temporary); first iApply "Hmono_Pastk1".
-        assert (a_stk1 ∈ finz.seq_between csp_b csp_e) as Hastk1_range.
-        { rewrite elem_of_finz_seq_between.
-          solve_addr+Hastk1 Hcsp_size' Hcsp_size.
-        }
-        clear -Hl_revoked_W0_nodup Hl_revoked_W0_temporaries Hastk1_range.
-        assert ( a_stk1 ∈ l_revoked_W0 ++ finz.seq_between csp_b csp_e ) as Ha.
-        { apply elem_of_app; right; done. }
-        by specialize (Hl_revoked_W0_temporaries a_stk1); apply Hl_revoked_W0_temporaries in Ha.
-      + (* apply Hwcond_Pastk1, but remove the later... *)
-        rewrite /=.
-        iApply "Hwcond_Pastk1'".
-        iApply interp_int.
-    }
-
-    (* Insert the allocated SO [a_stk1] in the world *)
-    iMod (world_interp_restore_world W2 W2 C [a_stk1] with
-      "[$Hworld_interp_C] [ Hastk1_closing_resources ]") as "Hworld_interp_C".
-    { apply close_list_related_sts_pub. }
-    { iClear "#".
-      iApply (big_sepL_impl with "Hastk1_closing_resources").
-      iModIntro; iIntros (k ka Hka) "(%&%&$&(%&$&$&?&$)&$)".
-      by rewrite mono_temporary_eq.
-    }
-    set (W3 := reinstate W2 _).
-    assert (related_sts_pub_world W2 W3) as Hrelated_pub_W2_W3.
-    { apply close_list_related_sts_pub. }
-    assert (related_sts_priv_world W0 W3) as Hrelated_priv_W0_W3.
-    { eapply related_sts_priv_pub_trans_world; eauto. }
-
-    assert (W0.1 !! a_stk1 = Some Temporary) as Ha_stk1_W0.
+    assert (std W0 !! a_stk1 = Some Temporary) as Ha_stk1_W0.
     { apply Hl_revoked_W0_temporaries.
       apply elem_of_app; right.
       apply elem_of_finz_seq_between; solve_addr+Hastk1 Hastk2 Hcsp_size Hcsp_size'.
     }
-    assert (W3.1 !! a_stk1 = Some Temporary) as Ha_stk1_W3.
-    {
-      apply close_list_lookup_in; last set_solver+.
+    assert (std W2 !! a_stk1 = Some Revoked) as Ha_stk1_W2.
+    { subst W2.
       rewrite close_list_lookup_not_in.
-      * cbn; apply revoke_lookup_Monotemp; done.
+      * subst W1; cbn. apply revoke_lookup_Monotemp. exact Ha_stk1_W0.
       * subst la_be_temporaries.
         intro Ha'.
-        rewrite elem_of_disjoint in H0; eapply H0; eauto.
+        rewrite elem_of_disjoint in Hstack_temps_disjoint.
+        eapply Hstack_temps_disjoint; eauto.
         apply elem_of_finz_seq_between; solve_addr+Hastk1 Hastk2 Hcsp_size Hcsp_size'.
     }
-    (* And show that the allocated SO is safe to share *)
-    iAssert (interp W3 C (WCap RWL Local a_stk1 a_stk2 a_stk1))%I
-      as "#Hinterp_W2_wca1".
-    {
-      iEval (rewrite fixpoint_interp1_eq interp1_eq).
-      cbn.
-      iSplit; last done.
-      rewrite (finz_seq_between_singleton a_stk1 a_stk2);last solve_addr+Hastk1 Hastk2 Hcsp_size.
-      cbn.
-      iSplit; last done.
-      iClear "∗".
-      iDestruct "Hinterp_W0_csp" as "-#Hinterp"; iClear "#".
-      iDestruct (read_allowed_inv _ _ a_stk1 with "Hinterp")
-        as "(%px & %Px & %Hpx_flow & %HPx_pers & Hrelx & Hzcondx & Hrcondx & Hwcondx & Hmonox)"; auto
-      ; first solve_addr+Hastk1 Hastk2 Hcsp_size Hcsp_size'.
-      iFrame "∗%".
-      apply readAllowed_flowsto in Hpx_flow; last done.
-      rewrite Hpx_flow; iFrame.
-      rewrite /monoReq.
-      rewrite Ha_stk1_W0 Ha_stk1_W3; done.
-    }
+    (* Update the world and insert [la_be_temporaries]. *)
+    set (W3 := reinstate W2 [a_stk1]).
+    (* Insert the allocated SO [a_stk1] in the world. *)
+    iMod (stack_object_reinstate_fresh_object
+      W0 W2 C csp_b csp_e csp_b a_stk1 a_stk2
+      with "[$Hinterp_W0_csp $Hworld_interp_C $Hastk1 $Hlc]")
+      as "(Hworld_interp_C & %Hrelated_pub_W2_W3
+           & %Ha_stk1_W3 & #Hinterp_W2_wca1)"; eauto.
+    { split; first solve_addr+Hastk1.
+      split; solve_addr+Hastk1 Hastk2 Hcsp_size Hcsp_size'. }
+    assert (related_sts_priv_world W0 W3) as Hrelated_priv_W0_W3.
+    { eapply related_sts_priv_pub_trans_world; eauto. }
     iDestruct (interp_monotone with "[] Hinterp_wca0_W2") as "Hinterp_wca0_W3"; eauto.
 
+    (* The passed object is safe to share in the world [W2]. *)
     iAssert (if is_sealed_with_o wca1 ot_switcher
              then (interp W3 C wca1)
              else True)%I as "#Hinterp_W3_wct1".
@@ -955,7 +482,7 @@ Section SO.
       }
       rewrite close_list_lookup_not_in.
       2: { intro Hx'.
-           apply H0 in Hx'; first done.
+           apply Hstack_temps_disjoint in Hx'; first done.
            apply elem_of_finz_seq_between in Hx.
            apply elem_of_finz_seq_between.
            solve_addr+Hx Hastk2 Hcsp_size' Hastk1 Hcsp_size.
@@ -975,11 +502,8 @@ Section SO.
     iMod ("Hso_code_close" with "[$Hna Himport_assert Himport_switcher Himport_C_f Himports_main $Hcode_main]")
       as "Hna".
     { iNext.
-      iDestruct (region_pointsto_cons with "[$Himport_C_f $Himports_main]") as "Himports_main"
-      ; [solve_addr|solve_addr|].
-      iDestruct (region_pointsto_cons with "[$Himport_assert $Himports_main]") as "Himports_main"
-      ; [solve_addr|solve_addr|].
-      iDestruct (region_pointsto_cons with "[$Himport_switcher $Himports_main]") as "$" ;solve_addr.
+      iApply so_main_imports_pointsto; first exact Hso_imports.
+      iFrame.
     }
 
     (* Apply the spec switcher call *)
@@ -1019,8 +543,10 @@ Section SO.
       apply HW3_revoked_callee_frm.
       rewrite !elem_of_finz_seq_between in Hx |- *; solve_addr+Hx.
     }
+    (* Derive a bunch of disjointness properties that will be necessary later. *)
     set (W5 := revoke W4).
-    (* Derive a bunch of disjointness properties that will be necessary later *)
+    (* Revoke the returned world resources by separation.  The repair helper
+       later uses these state facts to reconcile the two revocation sets. *)
     iMod (world_interp_revoked_by_separation_many_with_RevokedResources
            with "[$Hrevoked_l_revoked_W0_no_be $Hworld_interp_C]")
       as "(Hworld_interp_C & Hrevoked_l_revoked_W0_no_be & %Hrevoked_l_revoked_W0_no_be_W5)".
@@ -1087,25 +613,17 @@ Section SO.
     codefrag_facts "Hcode_main" ; rename H into Hpc_contiguous; clear H0.
 
     (* Extract the imports *)
-    iDestruct (region_pointsto_cons with "Himports_main") as "[Himport_switcher Himports_main]".
-    { transitivity (Some (pc_b ^+ 1)%a); auto; solve_addr. }
-    { solve_addr. }
-    iDestruct (region_pointsto_cons with "Himports_main") as "[Himport_assert Himports_main]".
-    { transitivity (Some (pc_b ^+ 2)%a); auto; solve_addr. }
-    { solve_addr. }
+    iDestruct (so_main_imports_pointsto with "Himports_main") as
+      "(Himport_switcher & Himport_assert & Himport_C_f & Himports_main)"; eauto.
 
     focus_block 10 "Hcode_main" as a_assert_prep Ha_assert_prep "Hcode" "Hcont"; iHide "Hcont" as hcont; clear dependent Ha_call.
 
-    (* Lea csp (-2)%Z *)
-    iInstr "Hcode".
-    { transitivity (Some csp_b); auto.
-      solve_addr+Hastk1 Hastk2 Hcsp_size Hcsp_size'.
-    }
-    (* Load ct0 csp *)
-    iInstr "Hcode".
-    { split;auto; solve_addr+Hcsp_size. }
-    (* Mov ct1 so_secret *)
-    iInstr "Hcode".
+    iApply (stack_object_assert_prep_block_spec
+              with "[- $HPC $Hcsp $Hct0 $Hct1 $Hastk0 $Hcode]").
+    { solve_addr+Hastk1 Hastk2. }
+    { eauto. }
+    iNext.
+    iIntros "(HPC & Hcsp & Hct0 & Hct1 & Hastk0 & Hcode)".
 
     subst hcont; unfocus_block "Hcode" "Hcont" as "Hcode_main".
 
@@ -1129,22 +647,17 @@ Section SO.
     (* ----------------- BLOCK 12: RETURN ----------------- *)
     (* --------------------------------------------------- *)
     focus_block 12 "Hcode_main" as a_halt Ha_halt "Hcode" "Hcont"; iHide "Hcont" as hcont ; clear dependent Ha_assert_c.
-    (* Mov cra cs0; *)
-    iInstr "Hcode".
-    (* Mov ca0 0%Z; *)
-    iInstr "Hcode".
-    (* Mov ca1 0%Z; *)
-    iInstr "Hcode".
-    (* Jalr cnull cra *)
-    iInstr "Hcode".
+    iApply (stack_object_return_block_spec
+              with "[- $HPC $Hcra $Hcs0 $Hca0 $Hca1 $Hcnull $Hcode]"); eauto.
+    iNext.
+    iIntros "(HPC & Hcra & Hcs0 & Hca0 & Hca1 & Hcnull & Hcode)".
     subst hcont; unfocus_block "Hcode" "Hcont" as "Hcode_main".
 
-    iMod ("Hso_code_close" with "[$Hna Himport_switcher Himport_assert Himports_main $Hcode_main]")
+    iMod ("Hso_code_close" with "[$Hna Himport_switcher Himport_assert Himport_C_f Himports_main $Hcode_main]")
       as "Hna".
     { iNext.
-      iDestruct (region_pointsto_cons with "[$Himport_assert $Himports_main]") as "Himports_main"
-      ; [solve_addr|solve_addr|].
-      iDestruct (region_pointsto_cons with "[$Himport_switcher $Himports_main]") as "$" ;solve_addr.
+      iApply so_main_imports_pointsto; first exact Hso_imports.
+      iFrame.
     }
 
     (* Put all the registers under the same map *)
@@ -1158,374 +671,59 @@ Section SO.
     iDestruct (big_sepM_insert _ _ cra with "[$Hrmap $Hcra]") as "Hrmap".
     { repeat (rewrite lookup_insert_ne; auto); apply not_elem_of_dom_1; rewrite Hdom_rmap ; set_solver+. }
 
-    assert (a_stk1 ∈ l_revoked_W4) as Hastk1_l_revoked_W4.
-    { assert (a_stk1 ∉ finz.seq_between (a_stk2 ^+ 4)%a csp_e).
-      {
-        apply not_elem_of_finz_seq_between.
-        solve_addr+Hcsp_bounds Hastk1 Hastk2 Hcsp_size' Hcsp_size.
-      }
-      clear -Hl_revoked_W4_temporaries Hrelated_pub_2ext_W4 H Ha_stk1_W3 H1.
-      assert (std W4 !! a_stk1 = Some Temporary) as Htemp.
-      { eapply region_state_pub_temp; eauto.
-        rewrite std_sta_update_multiple_lookup_same_i; auto.
-      }
-      apply Hl_revoked_W4_temporaries in Htemp.
-      apply elem_of_app in Htemp as [?|?]; done.
-    }
+    (* Repair the initial and returned revocation sets together.  The helper
+       removes the fresh cell and the incoming object overlap, closes the
+       repaired world, and reconstructs the complete stack region. *)
+    set (l_revoked_W4_no_astk1 :=
+      filter (fun a => a <> a_stk1) l_revoked_W4).
+    set (l_revoked_W4_no_astk1_wca0 :=
+      filter (fun a => a ∈ la_be_temporaries)
+        l_revoked_W4_no_astk1).
+    set (l_revoked_W4_no_astk1_no_wca0 :=
+      filter (fun a => a ∉ la_be_temporaries)
+        l_revoked_W4_no_astk1).
+    set (closing_list_revoked_addresses :=
+      l_revoked_W0 ++ l_revoked_W4_no_astk1_no_wca0).
+    set (closing_list :=
+      closing_list_revoked_addresses ++ finz.seq_between csp_b csp_e).
 
-    assert (∀ a, a ∈ l_revoked_W0 ++ finz.seq_between csp_b csp_e -> std (revoke W4) !! a = Some Revoked) as
-    Ha_5.
-    { clear a ; intros a Ha.
-      apply elem_of_app in Ha as [Ha|Ha]; cycle 1.
-      - rewrite finz_seq_between_cons in Ha; last solve_addr+Hcsp_size' Hastk1.
-        replace (csp_b ^+1)%a with a_stk1 in Ha by solve_addr+Hcsp_size' Hastk2 Hastk1 Hcsp_bounds.
-        rewrite finz_seq_between_cons in Ha; last solve_addr+Hcsp_size' Hastk1 Hcsp_bounds.
-        replace (a_stk1 ^+1)%a with a_stk2 in Ha by solve_addr+Hcsp_size' Hastk2 Hastk1 Hcsp_bounds.
-        apply elem_of_cons in Ha as [Ha | Ha]; simplify_eq; first auto.
-        apply elem_of_cons in Ha as [Ha | Ha]; simplify_eq.
-        { rewrite /revoked_addresses Forall_forall in Hl_revoked_W4; apply Hl_revoked_W4 in Hastk1_l_revoked_W4; auto. }
-        rewrite Forall_forall in Hstk_W5; apply Hstk_W5 in Ha; auto.
-      - setoid_rewrite Hl_wca0_l' in Ha.
-        apply elem_of_app in Ha as [Ha|Ha]; cycle 1.
-        + rewrite Forall_forall in Hrevoked_l_revoked_W0_no_be_W5; apply Hrevoked_l_revoked_W0_no_be_W5 in Ha; auto.
-        + apply revoke_lookup_Monotemp.
-          eapply region_state_pub_temp; eauto.
-          rewrite close_list_lookup_not_in; auto.
-          * rewrite close_list_lookup_in; auto.
-            rewrite Forall_forall in Hrevoked_la_be_temporaries; apply Hrevoked_la_be_temporaries; auto.
-          * intro Ha' ; apply list_elem_of_singleton in Ha'; simplify_eq.
-            apply list_elem_of_filter in Ha as [_ Ha].
-            rewrite elem_of_disjoint in Hno_overlap; eapply Hno_overlap; eauto.
-            apply elem_of_finz_seq_between; subst csp_b; solve_addr+Hastk1 Hcsp_size'.
-    }
+    iMod (stack_object_repair_world_for_return
+      W0 W3 W4 C b e csp_b csp_e a_stk1 a_stk2
+      l_revoked_W0 l_revoked_W4 (WInt so_secret) stk_mem
+      with "[$Hworld_interp_C $Hrevoked_l_revoked_W0_no_be
+             $Hl_revoked_W4 $Hastk0 $Hstk]")
+      as (w_stk1_return)
+        "(Hworld_interp_C & %Hrelated_pub_W0_Wfixed & %Hclosing_list_nodup
+          & %Hclosing_list_covers_W0 & Hrevoked & Hstk)".
+    { split; eauto. }
+    { split; eauto. }
+    { subst W3 W2 W1 la_be_temporaries. reflexivity. }
+    { exact Ha_stk1_W3. }
+    { exact Hrelated_priv_W0_W3. }
+    { exact Hrelated_pub_W3_W4. }
+    { exact Hno_overlap. }
+    { exact Hastk1. }
+    { exact Hastk2. }
+    { exact Hastk2_csp_e. }
+    { exact Hcsp_bounds. }
+    { exact Hl_revoked_W4. }
+    { exact Hrevoked_l_revoked_W0_no_be_W5. }
+    { exact Hstk_W5. }
+    { exact Hastk0_W5. }
 
-    (* To fix the world, we need to close the world with the addresses from
-       [l_revoked_W0] and [l_revoked_W4], but they have some overlap.
-       So we need to separe them into disjoint lists.
-     *)
-    iDestruct (RevokedResources_disjoint with "[$Hrevoked_l_revoked_W0_no_be $Hl_revoked_W4]") as "%Hdisjoint_l_revoked_W0_no_be_l_revoked_W4".
-    assert (∃ l_revoked_W4_no_astk1, l_revoked_W4 ≡ₚ a_stk1::l_revoked_W4_no_astk1 ∧ a_stk1 ∉ l_revoked_W4_no_astk1) as (l_revoked_W4_no_astk1 & Hl_revoked_W4_astk1 & Ha_stk1_l_revoked_W4_no_astk1).
-    {
-      clear -Hastk1_l_revoked_W4 Hl_revoked_W4_nodup.
-      apply elem_of_Permutation in Hastk1_l_revoked_W4.
-      destruct Hastk1_l_revoked_W4 as [l_revoked_W4_no_astk1 Hl_revoked_W4_no_astk1].
-      exists l_revoked_W4_no_astk1; split; first done.
-      setoid_rewrite Hl_revoked_W4_no_astk1 in Hl_revoked_W4_nodup.
-      apply NoDup_app in Hl_revoked_W4_nodup; destruct Hl_revoked_W4_nodup as (Hnodup & _ & _).
-      apply NoDup_cons in Hnodup; destruct Hnodup as [? _]; done.
-    }
-    iAssert (
-       RevokedResources W4 C l_revoked_W4_no_astk1
-       ∗ RevokedResources W4 C [a_stk1]
-      )%I with "[Hl_revoked_W4]" as "[Hl_revoked_W4 Ha_stk1]".
-    { setoid_rewrite Hl_revoked_W4_astk1.
-      replace (a_stk1 :: l_revoked_W4_no_astk1) with ( [a_stk1] ++ l_revoked_W4_no_astk1) by done.
-      iDestruct (RevokedResources_app with "Hl_revoked_W4") as "[$ $]".
-    }
-    set (l_revoked_W4_no_astk1_no_wca0 := filter (fun a => a ∉ la_be_temporaries) l_revoked_W4_no_astk1).
-    set (l_revoked_W4_no_astk1_wca0 := filter (fun a => a ∈ la_be_temporaries) l_revoked_W4_no_astk1).
-    assert (l_revoked_W4_no_astk1 ≡ₚ l_revoked_W4_no_astk1_wca0 ∪ l_revoked_W4_no_astk1_no_wca0) as Hl_revoked_W4_no_astk1_p.
-    { clear.
-      subst l_revoked_W4_no_astk1_wca0 l_revoked_W4_no_astk1_no_wca0.
-      apply filter_complement_list.
-    }
-    assert ( l_revoked_W0 ≡ₚ l_revoked_W0_no_be ∪ l_revoked_W4_no_astk1_wca0) as Hl_l_revoked_W4_no_astk1_wca0.
-    { subst l_revoked_W0_no_be l_revoked_W4_no_astk1_wca0 l_revoked_W4_no_astk1_no_wca0.
-      apply NoDup_app in Hl_revoked_W0_nodup as (Hnodup_l&?&?).
-      apply NoDup_app in Hl_revoked_W4_nodup as (Hl_revoked_W4_nodup&?&?).
-      eapply NoDup_Permutation; eauto.
-      { apply NoDup_app.
-        split;[|split]; try (apply NoDup_filter); auto; cycle 1.
-        + apply (NoDup_cons_1_2 a_stk1).
-          setoid_rewrite <- Hl_revoked_W4_astk1; auto.
-        + intros x Hx Hx'.
-          apply list_elem_of_filter in Hx as [Hx _].
-          apply list_elem_of_filter in Hx' as [Hx' _].
-          done.
-      }
-      intros x; split; intros Hx.
-      + apply elem_of_app.
-        destruct (decide (x ∈ la_be_temporaries)) as [Hx_temp|Hx_temp]; [right|left]; cycle 1.
-        * apply list_elem_of_filter; split; auto.
-        * apply list_elem_of_filter; split; auto.
-          assert (std W4 !! x = Some Temporary) as Hx_W4.
-          { eapply region_state_pub_temp; eauto.
-            destruct (decide (x ∈ [a_stk1])) as [Hx'|Hx'].
-            + rewrite list_elem_of_singleton in Hx'; simplify_eq; done.
-            + rewrite close_list_lookup_not_in; eauto.
-              apply close_list_lookup_in; eauto.
-              rewrite /revoked_addresses Forall_forall in Hl_revoked_W0; apply Hl_revoked_W0; auto.
-          }
-          apply list_elem_of_filter in Hx_temp as [Hx_temp_W0 Hx_temp].
-          subst la_be_temporaries.
-          apply Hl_revoked_W4_temporaries in Hx_W4.
-          apply elem_of_app in Hx_W4 as [Hx_W4|Hx_W4].
-          { setoid_rewrite Hl_revoked_W4_astk1 in Hx_W4.
-            apply elem_of_cons in Hx_W4 as [Hx_W4|Hx_W4]; last done; simplify_eq.
-            assert (a_stk1 ∈ finz.seq_between csp_b csp_e)
-              by (apply elem_of_finz_seq_between; solve_addr+Hastk1 Hcsp_size').
-            exfalso; rewrite elem_of_disjoint in Hno_overlap ; eapply Hno_overlap; eauto.
-          }
-          { apply elem_of_finz_seq_between in Hx_W4.
-            assert (x ∈ finz.seq_between csp_b csp_e)
-              by (apply elem_of_finz_seq_between; solve_addr+Hastk1 Hastk2 Hcsp_size' Hx_W4).
-            exfalso; rewrite elem_of_disjoint in Hno_overlap ; eapply Hno_overlap; eauto.
-          }
-      + apply elem_of_app in Hx as [Hx | Hx]
-        ; apply list_elem_of_filter in Hx as [Hx Hx']; first done.
-        assert (x ∈ finz.seq_between b e)
-          as Hx_be by (by apply list_elem_of_filter in Hx as [_ ?]).
-        assert ( W0.1 !! x = Some Temporary )
-          as Hx_W0 by (by apply list_elem_of_filter in Hx as [? _]).
-        apply Hl_revoked_W0_temporaries in Hx_W0.
-        apply elem_of_app in Hx_W0 as [Hx_W0|Hx_W0]; auto.
-            exfalso; rewrite elem_of_disjoint in Hno_overlap ; eapply Hno_overlap; eauto.
-    }
-
-    (* [closing_list_revoked_addresses] is the addresses revoked from [W0] and from [W4],
-       but without duplication *)
-    set (closing_list_revoked_addresses := l_revoked_W0++l_revoked_W4_no_astk1_no_wca0).
-    set (closing_list := (closing_list_revoked_addresses ++ finz.seq_between csp_b csp_e)).
-    (* Show that fixing the world [W4] with [closing_list] is public future world... *)
-    assert (related_sts_pub_world W4 (close_list closing_list W5)) as Hrelated_pub_W4_Wfixed.
-    { subst W5.
-      assert ( l_revoked_W4 ++ finz.seq_between (a_stk2 ^+ 4)%a csp_e ⊆ closing_list ).
-      { clear a.
-        intros a Ha.
-        apply elem_of_app in Ha as [Ha|Ha]; cycle 1.
-        { apply elem_of_app; right.
-          apply elem_of_finz_seq_between in Ha;
-          apply elem_of_finz_seq_between.
-          solve_addr+Ha Hcsp_bounds Hastk1 Hastk2.
-        }
-        setoid_rewrite Hl_revoked_W4_astk1 in Ha.
-        apply elem_of_cons in Ha as [Ha|Ha]; simplify_eq; cycle 1.
-        + apply elem_of_app; left.
-          subst closing_list_revoked_addresses.
-          setoid_rewrite Hl_l_revoked_W4_no_astk1_wca0.
-          rewrite -app_assoc.
-          setoid_rewrite <- Hl_revoked_W4_no_astk1_p.
-          apply elem_of_app; right.
-          done.
-        + apply elem_of_app; right.
-          rewrite elem_of_finz_seq_between; solve_addr+Hcsp_size' Hastk1.
-      }
-      destruct W4 as [W4std W4cus]; cbn.
-      split; cbn; last apply related_sts_pub_refl.
-      split; first (by setoid_rewrite <- close_list_dom_eq; setoid_rewrite <- revoke_dom_eq).
-      clear a.
-      intros a ρ4 ρ5 Ha_4 Ha_6.
-      destruct ρ4.
-      - (* Temporary in W4 *)
-        assert ( a ∈  l_revoked_W4 ++ finz.seq_between (a_stk2 ^+ 4)%a csp_e ) as Ha_closing.
-        { apply Hl_revoked_W4_temporaries; auto. }
-        rewrite close_list_std_sta_revoked in Ha_6; auto.
-        + simplify_eq; apply rtc_refl.
-        + by apply revoke_lookup_Monotemp.
-      - (* Permanent in W4 *)
-        apply revoke_lookup_Perm in Ha_4.
-        rewrite -close_list_std_sta_same_alt in Ha_6; [|intro]; simplify_eq.
-        apply rtc_refl.
-     - (* Revoked in W4 *)
-       destruct ρ5; try apply rtc_refl ; apply rtc_once; econstructor.
-    }
-    (* ... and use it for showing that we can close the resources of [l_revoked_W4_no_astk1] *)
-    iAssert (close_list_resources_gen C W5 closing_list l_revoked_W4_no_astk1 false) with "[Hl_revoked_W4]" as "Hl_revoked_W4".
-    { iApply close_list_resources_gen_eq; eauto.
-      rewrite world_ghost_theory.RevokedResources_eq.
-      done.
-    }
-
-    (* Show that fixing the world [W0] with [closing_list] is public future world... *)
-    assert (related_sts_pub_world W0 (close_list closing_list W5)) as Hrelated_pub_W0_Wfixed.
-    { subst W5.
-      assert ( l_revoked_W0 ++ finz.seq_between csp_b csp_e ⊆ closing_list ).
-      { clear a.
-        intros a Ha.
-        apply elem_of_app in Ha as [Ha|Ha]; last (by apply elem_of_app; right).
-         by do 2 (apply elem_of_app; left).
-      }
-      destruct W0 as [W0std W0cus]; cbn.
-      destruct W4 as [W4std W4cus]; cbn.
-      split; cbn; cycle 1.
-      { destruct Hrelated_priv_W0_W3 as [_ H_W0_W3].
-        destruct Hrelated_pub_W3_W4 as [_ H_W3_W4].
-        clear -H_W0_W3 H_W3_W4.
-        cbn in *.
-        eapply related_sts_pub_trans; eauto.
-        apply related_sts_pub_refl.
-      }
-      split.
-      {
-        destruct Hrelated_priv_W0_W3 as [ [H_W0_W3 _] _].
-        destruct Hrelated_pub_W3_W4 as [ [H_W3_W4 _] _].
-        clear -H_W0_W3 H_W3_W4.
-        setoid_rewrite <- close_list_dom_eq; setoid_rewrite <- revoke_dom_eq.
-        set_solver.
-      }
-      clear a.
-      intros a ρ0 ρ5 Ha_0 Ha_6.
-      destruct ρ0.
-      - (* Temporary in W0 *)
-        assert ( a ∈  l_revoked_W0 ++ finz.seq_between csp_b csp_e ) as Ha_closing.
-        { apply Hl_revoked_W0_temporaries; auto. }
-        assert (std W1 !! a = Some Revoked)
-          as Ha_1 by (by apply revoke_lookup_Monotemp).
-        specialize (Ha_5 a Ha_closing).
-        apply H in Ha_closing.
-        rewrite close_list_std_sta_revoked in Ha_6; auto.
-        simplify_eq; apply rtc_refl.
-      - (* Permanent in W0 *)
-        assert (std W3 !! a = Some Permanent) as Ha_3.
-        { eapply region_state_priv_perm; eauto. }
-        assert (std (W4std, W4cus) !! a = Some Permanent) as Ha_4.
-        { eapply region_state_priv_perm; eauto.
-          by apply related_sts_pub_priv_world.
-        }
-        apply revoke_lookup_Perm in Ha_4.
-        rewrite -close_list_std_sta_same_alt in Ha_6; [|intro Hcontra]; cbn; simplify_eq.
-        + rewrite Ha_4 in Ha_6; simplify_eq; apply rtc_refl.
-        + rewrite Ha_4 in Hcontra; done.
-      - (* Revoked in W0 *)
-        destruct ρ5; try apply rtc_refl ; apply rtc_once; econstructor.
-    }
-    (* ... and use it for showing that we can close the resources of [l_revoked_W0_no_be] *)
-    iAssert (close_list_resources_gen C W5 closing_list l_revoked_W0_no_be false) with "[Hrevoked_l_revoked_W0_no_be]" as "Hrevoked_l_revoked_W0_no_be".
-    { iApply close_list_resources_gen_eq; eauto.
-      rewrite world_ghost_theory.RevokedResources_eq.
-      done.
-    }
-
-    (* Derive some separation properties that will be requires later *)
-    iAssert (
-       close_list_resources_gen C W5 closing_list l_revoked_W4_no_astk1_no_wca0 false
-       ∗ close_list_resources_gen C W5 closing_list l_revoked_W4_no_astk1_wca0 false
-      )%I with "[Hl_revoked_W4]" as "[Hl_revoked_W4_no_wca0 Hl_revoked_W4_wca0]".
-    { rewrite /close_list_resources_gen.
-      setoid_rewrite Hl_revoked_W4_no_astk1_p.
-      iDestruct (big_sepL_app with "Hl_revoked_W4") as "[$ $]".
-    }
-    iDestruct (close_list_resources_gen_separation with "[$Hastk0] [$Hl_revoked_W4_no_wca0]") as "%Hcsp_b_notin_l_revoked_W4_no_astk1_no_wca0".
-    iDestruct (close_addr_list_gen_resources_separation with "[Ha_stk1] [$Hl_revoked_W4_no_wca0]") as "%Hastk_1_notin_l_revoked_W4_no_astk1_no_wca0".
-    { iClear "#".
-      rewrite /RevokedResources /close_addr_resources /=.
-      iDestruct "Ha_stk1" as "[ (%pa & %Pa & $ & $ & (%va & $ & $ & $ & ?)) _ ]".
-      by rewrite mono_temporary_eq.
-    }
-    iDestruct (close_list_resources_gen_separation_many
-                 with "[$Hstk] [$Hl_revoked_W4_no_wca0]") as "%Hfrm_notin_l_revoked_W4_no_astk1_no_wca0".
-    (* Combine all the revoked addresses [closing_list_revoked_addresses] that will
-     be used to fix the world *)
-    iAssert (close_list_resources_gen C W5 closing_list l_revoked_W0 false)
-      with "[Hrevoked_l_revoked_W0_no_be Hl_revoked_W4_wca0]" as "Hrevoked_l_revoked_W0_no_be".
-    { rewrite /close_list_resources_gen.
-      setoid_rewrite Hl_l_revoked_W4_no_astk1_wca0.
-      iApply big_sepL_app; iFrame.
-    }
-    iAssert (close_list_resources_gen C W5 closing_list closing_list_revoked_addresses false)
-      with "[Hrevoked_l_revoked_W0_no_be Hl_revoked_W4_no_wca0]" as "Hrevoked".
-    { rewrite /close_list_resources_gen; iApply big_sepL_app; iFrame. }
-
-    (* Reconstruct the stack region *)
-    iDestruct "Ha_stk1" as "[ (%pa & %Pa & _ & _ & (%va & _ & Ha_stk1 & _ & _)) _ ]".
-    iDestruct (region_pointsto_cons with "[$Ha_stk1 $Hstk]") as "Hstk"; auto.
-    { solve_addr+Hcsp_size' Hastk2. }
-    iDestruct (region_pointsto_cons with "[$Hastk0 $Hstk]") as "Hstk"; auto.
-    { solve_addr+Hcsp_size Hastk1. }
-
-    (* Apply the generalised version of the return to switcher specification *)
+    (* The repair helper's postcondition is exactly the generalized switcher
+       return protocol: no filtering or resource surgery remains here. *)
     iApply (switcher_ret_specification_gen _ W0 W5
              with
              "[ $Hswitcher $Hstk $Hcstk_frag $HK $Hworld_interp_C $Hna $HPC
-             $Hrmap $Hca0 $Hca1 $Hcsp $Hrevoked]"
-           ); eauto.
+                $Hrmap $Hca0 $Hca1 $Hcsp $Hrevoked]"); eauto.
     { repeat (rewrite dom_insert_L); rewrite Hdom_rmap; set_solver+. }
     { subst csp_b.
       clear -Hsync_csp.
       destruct Hsync_csp as [].
-      rewrite -H0; auto.
-    }
-    {
-      apply NoDup_app.
-      split;[|split]; cycle -1.
-      - apply finz_seq_between_NoDup.
-      - subst closing_list_revoked_addresses.
-        setoid_rewrite Hl_l_revoked_W4_no_astk1_wca0.
-        subst l_revoked_W0_no_be.
-        rewrite /union /Union_list.
-        apply NoDup_app.
-        split;[|split]; cycle -1.
-        + subst l_revoked_W4_no_astk1_no_wca0.
-          apply NoDup_filter.
-          clear -Hl_revoked_W4_nodup Hl_revoked_W4_astk1.
-          apply NoDup_app in Hl_revoked_W4_nodup as (Hnodup&_&_).
-          setoid_rewrite Hl_revoked_W4_astk1 in Hnodup.
-          apply NoDup_cons in Hnodup as [_ Hnodup].
-          done.
-        + apply NoDup_app.
-          split;[|split]; cycle -1.
-          * subst l_revoked_W4_no_astk1_wca0.
-            apply NoDup_filter.
-            clear -Hl_revoked_W4_nodup Hl_revoked_W4_astk1.
-            apply NoDup_app in Hl_revoked_W4_nodup as (Hnodup&_&_).
-            setoid_rewrite Hl_revoked_W4_astk1 in Hnodup.
-            apply NoDup_cons in Hnodup as [_ Hnodup].
-            done.
-          * apply NoDup_filter.
-            clear -Hl_revoked_W0_nodup Hl_revoked_W0_temporaries.
-            apply NoDup_app in Hl_revoked_W0_nodup as (Hl_revoked_W0_nodup&_&_).
-            done.
-          * cbn; intros x Hx.
-            clear -Hx.
-            apply list_elem_of_filter in Hx as [Hx _].
-            subst l_revoked_W4_no_astk1_wca0.
-            intros Hx'.
-            apply list_elem_of_filter in Hx' as [Hx' _].
-            done.
-        + cbn; intros x Hx.
-          intros Hx'.
-          subst l_revoked_W4_no_astk1_no_wca0.
-          apply list_elem_of_filter in Hx' as [Hx_no_la_be_temporaries Hx'].
-          apply elem_of_app in Hx as [Hx|Hx].
-          * apply list_elem_of_filter in Hx as [_ Hx].
-            apply (list_elem_of_further _ a_stk1) in Hx'.
-            setoid_rewrite <- Hl_revoked_W4_astk1 in Hx'.
-            setoid_rewrite Hl_wca0_l' in Hx.
-            clear -Hx Hx_no_la_be_temporaries Hx' Hdisjoint_l_revoked_W0_no_be_l_revoked_W4.
-            rewrite elem_of_disjoint in Hdisjoint_l_revoked_W0_no_be_l_revoked_W4.
-            apply elem_of_app in Hx as [Hx|Hx]; first done.
-            apply (Hdisjoint_l_revoked_W0_no_be_l_revoked_W4 x); eauto.
-          * subst l_revoked_W4_no_astk1_wca0.
-            apply list_elem_of_filter in Hx as [Hx _].
-            done.
-      - cbn; intros x Hx.
-        apply elem_of_app in Hx as [Hx|Hx].
-        + clear -Hx Hl_revoked_W0_nodup Hl_revoked_W0_temporaries.
-          apply NoDup_app in Hl_revoked_W0_nodup as (_&Hl_revoked_W0_nodup&_).
-          by apply Hl_revoked_W0_nodup.
-        + rewrite finz_seq_between_cons; last solve_addr+Hcsp_bounds Hastk1 Hastk2.
-          apply not_elem_of_cons; split.
-          { intros ->; done. }
-          replace (csp_b ^+ 1)%a with a_stk1; last solve_addr+Hcsp_bounds Hastk1 Hastk2.
-          rewrite finz_seq_between_cons; last solve_addr+Hcsp_bounds Hastk1 Hastk2.
-          apply not_elem_of_cons; split.
-          { intros ->; done. }
-          replace (a_stk1 ^+ 1)%a with a_stk2; last solve_addr+Hcsp_bounds Hastk1 Hastk2.
-          intro Hx'.
-          rewrite elem_of_disjoint in Hfrm_notin_l_revoked_W4_no_astk1_no_wca0.
-          eapply Hfrm_notin_l_revoked_W4_no_astk1_no_wca0; eauto.
-    }
-    {
-    intros x.
-    specialize (Hl_revoked_W0_temporaries x).
-    intros Hx.
-    apply Hl_revoked_W0_temporaries in Hx.
-    apply elem_of_app in Hx as [Hx | Hx].
-    * apply elem_of_app; left.
-      apply elem_of_app; left; done.
-    * apply elem_of_app; right; done.
-    }
+      rewrite -H0; auto. }
     { iSplit; iApply interp_int. }
+
   Qed.
 
 
